uniform notation and equiavariance inference for all rule induction instances

thys/POPLmark/POPLmark_1A.thy
@@ -1,598 +1,6 @@
 theory POPLmark_1A
-  imports "../MRBNF_Recursor"
-    "../Instantiation_Infrastructure/Curry_LFP"
-    "../Generic_Barendregt_Enhanced_Rule_Induction"
-    "../Instantiation_Infrastructure/FixedCountableVars"
+imports SystemFSub
 begin
-
-declare bij_swap[simp]
-declare supp_id_bound[simp]
-
-ML \<open>
-val ctors = [
-  (("TyVar", (NONE : mixfix option)), [@{typ 'var}]),
-  (("Top", (NONE : mixfix option)), []),
-  (("Fun", NONE), [@{typ 'rec}, @{typ 'rec}]),
-  (("Forall", NONE), [@{typ 'bvar}, @{typ 'rec}, @{typ 'brec}])
-]
-
-val spec = {
-  fp_b = @{binding "typ"},
-  vars = [
-    (dest_TFree @{typ 'var}, MRBNF_Def.Free_Var),
-    (dest_TFree @{typ 'bvar}, MRBNF_Def.Bound_Var),
-    (dest_TFree @{typ 'brec}, MRBNF_Def.Live_Var),
-    (dest_TFree @{typ 'rec}, MRBNF_Def.Live_Var)
-  ],
-  binding_rel = [[0]],
-  rec_vars = 2,
-  ctors = ctors,
-  map_b = @{binding vvsubst_typ},
-  tvsubst_b = @{binding tvsubst_typ}
-}
-\<close>
-
-declare [[mrbnf_internals]]
-local_setup \<open>fn lthy =>
-let
-  val lthy' = MRBNF_Sugar.create_binder_datatype spec lthy
-in lthy' end\<close>
-print_theorems
-print_mrbnfs
-
-instance var :: var_typ_pre apply standard
-  using Field_natLeq infinite_iff_card_of_nat infinite_var
-  by (auto simp add: regularCard_var)
-
-declare supp_swap_bound[OF cinfinite_imp_infinite[OF typ.UNIV_cinfinite], simp]
-declare typ.rrename_ids[simp] typ.rrename_id0s[simp]
-
-lemma rrename_typ_simps[simp]:
-  fixes f::"'a::var_typ_pre \<Rightarrow> 'a"
-  assumes "bij f" "|supp f| <o |UNIV::'a set|"
-  shows
-    "rrename_typ f (TyVar a) = TyVar (f a)"
-    "rrename_typ f Top = Top"
-    "rrename_typ f (Fun t1 t2) = Fun (rrename_typ f t1) (rrename_typ f t2)"
-    "rrename_typ f (Forall x T1 T2) = Forall (f x) (rrename_typ f T1) (rrename_typ f T2)"
-     apply (unfold TyVar_def Top_def Fun_def Forall_def)
-     apply (rule trans)
-      apply (rule typ.rrename_cctors)
-       apply (rule assms)+
-     defer
-     apply (rule trans)
-      apply (rule typ.rrename_cctors)
-       apply (rule assms)+
-     defer
-     apply (rule trans)
-      apply (rule typ.rrename_cctors)
-       apply (rule assms)+
-     defer
-     apply (rule trans)
-      apply (rule typ.rrename_cctors)
-       apply (rule assms)+
-     defer
-     apply (unfold map_typ_pre_def comp_def Abs_typ_pre_inverse[OF UNIV_I] map_sum.simps
-        map_prod_simp id_def
-      )
-     apply (rule refl)+
-  done
-
-lemma typ_inject:
-  "TyVar x = TyVar y \<longleftrightarrow> x = y"
-  "Fun T1 T2 = Fun R1 R2 \<longleftrightarrow> T1 = R1 \<and> T2 = R2"
-  "Forall x T1 T2 = Forall y R1 R2 \<longleftrightarrow> T1 = R1 \<and> (\<exists>f. bij (f::'a::var_typ_pre \<Rightarrow> 'a) \<and> |supp f| <o |UNIV::'a set| \<and> id_on (FFVars_typ T2 - {x}) f \<and> f x = y \<and> rrename_typ f T2 = R2)"
-    apply (unfold TyVar_def Fun_def Forall_def typ.TT_injects0
-      set3_typ_pre_def comp_def Abs_typ_pre_inverse[OF UNIV_I] map_sum.simps sum_set_simps
-      cSup_singleton Un_empty_left Un_empty_right Union_empty image_empty empty_Diff map_typ_pre_def
-      prod.map_id set2_typ_pre_def prod_set_simps prod.set_map UN_single Abs_typ_pre_inject[OF UNIV_I UNIV_I]
-      sum.inject prod.inject map_prod_simp
-    )
-  by auto
-declare typ_inject(1,2)[simp]
-
-corollary Forall_inject_same[simp]: "Forall x T1 T2 = Forall x R1 R2 \<longleftrightarrow> T1 = R1 \<and> T2 = R2"
-  using typ_inject(3) typ.rrename_cong_ids
-  by (metis (no_types, lifting) Diff_empty Diff_insert0 id_on_insert insert_Diff)
-
-lemma Forall_rrename:
-  assumes "bij \<sigma>" "|supp \<sigma>| <o |UNIV::'a set|" shows "
- (\<And>a'. a'\<in>FFVars_typ T2 - {x::'a::var_typ_pre} \<Longrightarrow> \<sigma> a' = a') \<Longrightarrow> Forall x T1 T2 = Forall (\<sigma> x) T1 (rrename_typ \<sigma> T2)"
-  apply (unfold Forall_def)
-  apply (unfold typ.TT_injects0)
-  apply (unfold set3_typ_pre_def set2_typ_pre_def comp_def Abs_typ_pre_inverse[OF UNIV_I] map_sum.simps
-    map_prod_simp sum_set_simps prod_set_simps cSup_singleton Un_empty_left Un_empty_right
-    Union_empty image_insert image_empty map_typ_pre_def id_def)
-  apply (rule exI[of _ \<sigma>])
-  apply (rule conjI assms)+
-   apply (unfold id_on_def atomize_all atomize_imp)[1]
-   apply (rule impI)
-   apply assumption
-  apply (rule refl)
-  done
-
-lemma Forall_swap: "y \<notin> FFVars_typ T2 - {x} \<Longrightarrow> Forall (x::'a::var_typ_pre) T1 T2 = Forall y T1 (rrename_typ (id(x:=y,y:=x)) T2)"
-  apply (rule trans)
-   apply (rule Forall_rrename)
-     apply (rule bij_swap[of x y])
-    apply (rule supp_swap_bound)
-    apply (rule cinfinite_imp_infinite[OF typ.UNIV_cinfinite])
-  by auto
-
-
-type_synonym type = "var typ"
-type_synonym \<Gamma>\<^sub>\<tau> = "(var \<times> type) list"
-
-definition map_context :: "(var \<Rightarrow> var) \<Rightarrow> \<Gamma>\<^sub>\<tau> \<Rightarrow> \<Gamma>\<^sub>\<tau>" where
-  "map_context f \<equiv> map (map_prod f (rrename_typ f))"
-
-abbreviation FFVars_ctxt :: "\<Gamma>\<^sub>\<tau> \<Rightarrow> var set" where
-  "FFVars_ctxt xs \<equiv> \<Union>(FFVars_typ ` snd ` set xs)"
-abbreviation extend :: "\<Gamma>\<^sub>\<tau> \<Rightarrow> var \<Rightarrow> type \<Rightarrow> \<Gamma>\<^sub>\<tau>" ("_ , _ <: _" [57,75,75] 71) where
-  "extend \<Gamma> x T \<equiv> (x, T)#\<Gamma>"
-abbreviation concat :: "\<Gamma>\<^sub>\<tau> \<Rightarrow> \<Gamma>\<^sub>\<tau> \<Rightarrow> \<Gamma>\<^sub>\<tau>" (infixl "(,)" 71) where
-  "concat \<Gamma> \<Delta> \<equiv> \<Delta> @ \<Gamma>"
-abbreviation empty_context :: "\<Gamma>\<^sub>\<tau>" ("\<emptyset>") where "empty_context \<equiv> []"
-abbreviation dom :: "\<Gamma>\<^sub>\<tau> \<Rightarrow> var set" where "dom xs \<equiv> fst ` set xs"
-abbreviation disjoint :: "\<Gamma>\<^sub>\<tau> \<Rightarrow> \<Gamma>\<^sub>\<tau> \<Rightarrow> bool" (infixl "(\<bottom>)" 71) where
-  "disjoint \<Gamma> \<Delta> \<equiv> dom \<Gamma> \<inter> dom \<Delta> = {}"
-
-lemma map_context_id[simp]: "map_context id = id"
-  unfolding map_context_def by simp
-lemma map_context_comp0[simp]:
-  assumes "bij f" "|supp f| <o |UNIV::var set|" "bij g" "|supp g| <o |UNIV::var set|"
-  shows "map_context f \<circ> map_context g = map_context (f \<circ> g)"
-  apply (rule ext)
-  unfolding map_context_def
-  using assms by (auto simp: typ.rrename_comps)
-lemmas map_context_comp = trans[OF comp_apply[symmetric] fun_cong[OF map_context_comp0]]
-declare map_context_comp[simp]
-lemma context_dom_set[simp]:
-  assumes "bij f" "|supp f| <o |UNIV::var set|"
-  shows "dom (map_context f xs) = f ` dom xs"
-  unfolding map_context_def by force
-lemma set_bd_UNIV: "|set xs| <o |UNIV::var set|"
-  apply (rule ordLess_ordLeq_trans)
-    apply (tactic \<open>resolve_tac @{context} (BNF_Def.set_bd_of_bnf (the (BNF_Def.bnf_of @{context} @{type_name list}))) 1\<close>)
-  apply (rule var_typ_pre_class.large)
-  done
-lemma context_set_bd_UNIV[simp]: "|dom xs| <o |UNIV::var set|"
-  apply (rule ordLeq_ordLess_trans[OF card_of_image])
-  apply (rule set_bd_UNIV)
-  done
-lemma context_map_cong_id:
-  assumes "bij f" "|supp f| <o |UNIV::var set|"
-  and "\<And>a. a \<in> dom \<Gamma> \<union> FFVars_ctxt \<Gamma> \<Longrightarrow> f a = a"
-shows "map_context f \<Gamma> = \<Gamma>"
-  unfolding map_context_def
-  apply (rule trans)
-   apply (rule list.map_cong0[of _ _ id])
-   apply (rule trans)
-    apply (rule prod.map_cong0[of _ _ id _ id])
-  using assms by (fastforce intro!: typ.rrename_cong_ids)+
-
-declare [[inductive_internals]]
-
-notation Fun (infixr "\<rightarrow>" 65)
-notation Forall ("\<forall> _ <: _ . _" [62, 62, 62] 70)
-
-abbreviation in_context :: "var \<Rightarrow> type \<Rightarrow> \<Gamma>\<^sub>\<tau> \<Rightarrow> bool" ("_ <: _ \<in> _" [55,55,55] 60) where
-  "x <: t \<in> \<Gamma> \<equiv> (x, t) \<in> set \<Gamma>"
-abbreviation well_scoped :: "type \<Rightarrow> \<Gamma>\<^sub>\<tau> \<Rightarrow> bool" ("_ closed'_in _" [55, 55] 60) where
-  "well_scoped S \<Gamma> \<equiv> FFVars_typ S \<subseteq> dom \<Gamma>"
-
-inductive wf_Ty :: "\<Gamma>\<^sub>\<tau> \<Rightarrow> bool" ("\<turnstile> _ ok" [70] 100) where
-  wf_Nil[intro]: "\<turnstile> [] ok"
-| wf_Cons[intro!]: "\<lbrakk> x \<notin> dom \<Gamma> ; T closed_in \<Gamma> ; \<turnstile> \<Gamma> ok \<rbrakk> \<Longrightarrow> \<turnstile> \<Gamma>,x<:T ok"
-
-inductive_cases
-  wfE[elim]: "\<turnstile> \<Gamma> ok"
-  and wf_ConsE[elim!]: "\<turnstile> (a#\<Gamma>) ok"
-print_theorems
-
-inductive Ty :: "\<Gamma>\<^sub>\<tau> \<Rightarrow> type \<Rightarrow> type \<Rightarrow> bool" ("_ \<turnstile> _ <: _" [55,55,55] 60) where
-  SA_Top: "\<lbrakk> \<turnstile> \<Gamma> ok ; S closed_in \<Gamma> \<rbrakk> \<Longrightarrow> \<Gamma> \<turnstile> S <: Top"
-| SA_Refl_TVar: "\<lbrakk> \<turnstile> \<Gamma> ok ; TyVar x closed_in \<Gamma> \<rbrakk> \<Longrightarrow> \<Gamma> \<turnstile> TyVar x <: TyVar x"
-| SA_Trans_TVar: "\<lbrakk> x<:U \<in> \<Gamma> ; \<Gamma> \<turnstile> U <: T \<rbrakk> \<Longrightarrow> \<Gamma> \<turnstile> TyVar x <: T"
-| SA_Arrow: "\<lbrakk> \<Gamma> \<turnstile> T\<^sub>1 <: S\<^sub>1 ; \<Gamma> \<turnstile> S\<^sub>2 <: T\<^sub>2 \<rbrakk> \<Longrightarrow> \<Gamma> \<turnstile> S\<^sub>1 \<rightarrow> S\<^sub>2 <: T\<^sub>1 \<rightarrow> T\<^sub>2"
-| SA_All: "\<lbrakk> \<Gamma> \<turnstile> T\<^sub>1 <: S\<^sub>1 ; \<Gamma>, x<:T\<^sub>1 \<turnstile> S\<^sub>2 <: T\<^sub>2 \<rbrakk> \<Longrightarrow> \<Gamma> \<turnstile> \<forall>x<:S\<^sub>1. S\<^sub>2 <: \<forall>x<:T\<^sub>1 .T\<^sub>2"
-
-inductive_cases
-  SA_TopE[elim!]: "\<Gamma> \<turnstile> Top <: T"
-and
-  SA_TVarE: "\<Gamma> \<turnstile> S <: TyVar Z"
-and
-  SA_ArrER: "\<Gamma> \<turnstile> S <: T\<^sub>1 \<rightarrow> T\<^sub>2"
-and
-  SA_ArrEL: "\<Gamma> \<turnstile> S\<^sub>1 \<rightarrow> S\<^sub>2 <: T "
-and
-  SA_AllER: "\<Gamma> \<turnstile> S <: \<forall>Z<:T\<^sub>1. T\<^sub>2"
-and
-  SA_AllEL: "\<Gamma> \<turnstile> \<forall>Z<:S\<^sub>1. S\<^sub>2 <: T "
-
-lemma wf_context: "\<Gamma> \<turnstile> S <: T \<Longrightarrow> \<turnstile> \<Gamma> ok"
-  by (induction \<Gamma> S T rule: Ty.induct)
-
-lemma well_scoped:
-  assumes "\<Gamma> \<turnstile> S <: T"
-  shows "S closed_in \<Gamma>" "T closed_in \<Gamma>"
-using assms proof (induction \<Gamma> S T rule: Ty.induct)
-case (SA_Trans_TVar x U \<Gamma> T) {
-  case 1 then show ?case using SA_Trans_TVar
-    by (metis fst_conv imageI singletonD subsetI typ.set(1))
-next
-  case 2 then show ?case using SA_Trans_TVar by simp
-} qed auto
-
-thm Ty_def
-declare Ty.intros[intro]
-
-(* instantiating the induction locale *)
-interpretation Small where dummy = "undefined :: var"
-apply standard
-  apply (simp add: infinite_var)
-  using var_typ_pre_class.regular by blast
-
-type_synonym T = "\<Gamma>\<^sub>\<tau> \<times> type \<times> type"
-type_synonym V = "var list"
-
-definition Tmap :: "(var \<Rightarrow> var) \<Rightarrow> T \<Rightarrow> T" where
-  "Tmap f \<equiv> map_prod (map_context f) (map_prod (rrename_typ f) (rrename_typ f))"
-fun Tfvars :: "T \<Rightarrow> var set" where
-  "Tfvars (\<Gamma>, T\<^sub>1, T\<^sub>2) = dom \<Gamma> \<union> FFVars_ctxt \<Gamma> \<union> FFVars_typ T\<^sub>1 \<union> FFVars_typ T\<^sub>2"
-
-(* definition Vmap :: "(var \<Rightarrow> var) \<Rightarrow> V \<Rightarrow> V" where
-  "Vmap \<equiv> map"
-fun Vfvars :: "V \<Rightarrow> var set" where
-  "Vfvars v = set v"
-*)
-
-interpretation Components where dummy = "undefined :: var" and
-Tmap = Tmap and Tfvars = Tfvars
-apply standard unfolding ssbij_def Tmap_def 
-  using small_Un small_def typ.card_of_FFVars_bounds
-         apply (auto simp: typ.FFVars_rrenames map_prod.comp typ.rrename_comp0s inf_A)
-    apply (rule var_typ_pre_class.Un_bound var_typ_pre_class.UN_bound context_set_bd_UNIV set_bd_UNIV
-        typ.card_of_FFVars_bounds)+
-      apply (auto simp: context_map_cong_id typ.rrename_cong_ids intro: context_map_cong_id)
-    apply (smt (verit, del_insts) UnI1 fst_conv imageI)
-  apply (unfold map_context_def)[1]
-   apply (smt (verit, del_insts) UN_I UnI1 UnI2 image_iff list.set_map prod_fun_imageE snd_conv typ.FFVars_rrenames)
-  done
-
-(* AtoJ: I have now removed the extra hypotheses for G, since 
-we are using the "enhanced" version *)
-definition G :: "(T \<Rightarrow> bool) \<Rightarrow> var set \<Rightarrow> T \<Rightarrow> bool" where
-  "G \<equiv> \<lambda>R B t.
-    (B = {} \<and> snd (snd t) = Top \<and> \<turnstile> fst t ok \<and> fst (snd t) closed_in fst t)
-  \<or> (\<exists>x. B = {} \<and> fst (snd t) = TyVar x \<and> fst (snd t) = snd (snd t) \<and> \<turnstile> fst t ok \<and> fst (snd t) closed_in fst t)
-  \<or> (\<exists>x U \<Gamma> T. B = {} \<and> fst t = \<Gamma> \<and> fst (snd t) = TyVar x \<and> snd (snd t) = T \<and> x <: U \<in> \<Gamma> \<and> R (\<Gamma>, U, T) 
-   \<comment> \<open>\<and> \<Gamma> \<turnstile> U <: T\<close>)
-  \<or> (\<exists>\<Gamma> T\<^sub>1 S\<^sub>1 S\<^sub>2 T\<^sub>2. B = {} \<and> fst t = \<Gamma> \<and> fst (snd t) = (S\<^sub>1 \<rightarrow> S\<^sub>2) \<and> snd (snd t) = (T\<^sub>1 \<rightarrow> T\<^sub>2) \<and> 
-     R (\<Gamma>, T\<^sub>1, S\<^sub>1) \<comment> \<open> \<and> \<Gamma> \<turnstile> T1 <: S1 \<close> \<and> 
-     R (\<Gamma>, S\<^sub>2, T\<^sub>2) \<comment> \<open> \<and> \<Gamma> \<turnstile> S2 <: T2 \<close> )
-  \<or> (\<exists>\<Gamma> T\<^sub>1 S\<^sub>1 x S\<^sub>2 T\<^sub>2. B = {x} \<and> fst t = \<Gamma> \<and> fst (snd t) = (\<forall>x<:S\<^sub>1. S\<^sub>2) \<and> snd (snd t) = (\<forall>x<:T\<^sub>1. T\<^sub>2) \<and> 
-     R (\<Gamma>, T\<^sub>1, S\<^sub>1) \<comment> \<open>\<and> \<Gamma> \<turnstile> T1 <: S1 \<close> \<and> 
-     R (\<Gamma>,x<:T\<^sub>1, S\<^sub>2, T\<^sub>2) \<comment> \<open>\<and> \<Gamma>,x<:T1 \<turnstile> S2 <: T2 \<close>)
-  "
-
-lemma G_mono: "R \<le> R' \<Longrightarrow> G R v t \<Longrightarrow> G R' v t"
-  unfolding G_def by fastforce
-
-lemma in_context_eqvt:
-  assumes "bij f" "|supp f| <o |UNIV::var set|"
-  shows "x <: T \<in> \<Gamma> \<Longrightarrow> f x <: rrename_typ f T \<in> map_context f \<Gamma>"
-  using assms unfolding map_context_def by auto
-
-lemma extend_eqvt:
-  assumes "bij f" "|supp f| <o |UNIV::var set|"
-  shows "map_context f (\<Gamma>,x<:T) = map_context f \<Gamma>,f x <: rrename_typ f T"
-  using assms unfolding map_context_def by simp
-
-lemma closed_in_eqvt:
-  assumes "bij f" "|supp f| <o |UNIV::var set|"
-  shows "S closed_in \<Gamma> \<Longrightarrow> rrename_typ f S closed_in map_context f \<Gamma>"
-  using assms by (auto simp: typ.FFVars_rrenames)
-
-lemma wf_eqvt:
-  assumes "bij f" "|supp f| <o |UNIV::var set|"
-  shows "\<turnstile> \<Gamma> ok \<Longrightarrow> \<turnstile> map_context f \<Gamma> ok"
-unfolding map_context_def proof (induction \<Gamma>)
-  case (Cons a \<Gamma>)
-  then show ?case using assms
-    by (smt (verit) Product_Type.fst_comp_map_prod image_comp image_mono list.discI list.inject list.set_map list.simps(9) map_prod_simp not_imageI typ.FFVars_rrenames wf_Cons wf_Ty.cases)
-qed simp
-
-lemma Ty_eqvt:
-  assumes "\<Gamma> \<turnstile> S <: T" "bij f" "|supp f| <o |UNIV::var set|"
-  shows "map_context f \<Gamma> \<turnstile> rrename_typ f S <: rrename_typ f T"
-  using assms proof (induction \<Gamma> S T rule: Ty.induct)
-  case (SA_Top \<Gamma> S)
-  then show ?case by (auto intro!: Ty.SA_Top dest: wf_eqvt closed_in_eqvt)
-next
-  case (SA_Refl_TVar \<Gamma> x)
-  then show ?case
-    apply (auto intro!: Ty.SA_Refl_TVar imageI dest: wf_eqvt closed_in_eqvt)
-    by (metis fst_conv image_iff)
-next
-  case (SA_Trans_TVar x U \<Gamma> T)
-  then show ?case by (auto intro!: Ty.SA_Trans_TVar dest: in_context_eqvt)
-next
-  case (SA_All \<Gamma> T\<^sub>1 S\<^sub>1 x S\<^sub>2 T\<^sub>2)
-  then show ?case by (auto intro!: Ty.SA_All simp: extend_eqvt)
-qed auto
-
-lemma G_equiv: "ssbij \<sigma> \<Longrightarrow> small B \<Longrightarrow> G R B t \<Longrightarrow> G (\<lambda>t'. R (Tmap (inv \<sigma>) t')) (image \<sigma> B) (Tmap \<sigma> t)"
-  unfolding G_def
-  apply (elim disjE)
-  subgoal
-    apply (rule disjI1)
-    apply (cases t)
-    unfolding ssbij_def Tmap_def using closed_in_eqvt wf_eqvt by simp
-  subgoal
-    apply (rule disjI2, rule disjI1)
-    apply (erule exE)
-    apply (elim conjE)
-    subgoal for x
-      apply (cases t)
-      unfolding ssbij_def Tmap_def using wf_eqvt by auto
-    done
-  subgoal
-    apply (rule disjI2, rule disjI2, rule disjI1)
-    apply (elim exE conjE)
-    subgoal for x U \<Gamma> T
-      apply (rule exI)
-      apply (rule exI[of _ "rrename_typ \<sigma> U"])
-      apply (rule exI[of _ "map_context \<sigma> \<Gamma>"])
-      apply (rule exI[of _ "rrename_typ \<sigma> T"])
-      apply (cases t)
-      unfolding ssbij_def Tmap_def 
-      apply (auto simp: in_context_eqvt supp_inv_bound typ.rrename_comps typ.rrename_comp0s Ty_eqvt)
-      done
-    done
-  subgoal
-    apply (rule disjI2, rule disjI2, rule disjI2, rule disjI1)
-    apply (elim exE conjE)
-    subgoal for \<Gamma> T1 S1 S2 T2
-      apply (rule exI[of _ "map_context \<sigma> \<Gamma>"])
-      apply (rule exI[of _ "rrename_typ \<sigma> T1"])
-      apply (rule exI[of _ "rrename_typ \<sigma> S1"])
-      apply (rule exI[of _ "rrename_typ \<sigma> S2"])
-      apply (rule exI[of _ "rrename_typ \<sigma> T2"])
-      apply (cases t) unfolding ssbij_def Tmap_def 
-      by (auto simp: in_context_eqvt supp_inv_bound
-          typ.rrename_comps typ.rrename_comp0s Ty_eqvt)
-    done
-  apply (rule disjI2)+
-  apply (elim exE conjE)
-  subgoal for \<Gamma> T1 S1 x S2 T2
-          apply (rule exI[of _ "map_context \<sigma> \<Gamma>"])
-      apply (rule exI[of _ "rrename_typ \<sigma> T1"])
-    apply (rule exI[of _ "rrename_typ \<sigma> S1"])
-    apply (rule exI)
-      apply (rule exI[of _ "rrename_typ \<sigma> S2"])
-    apply (rule exI[of _ "rrename_typ \<sigma> T2"])
-    apply (cases t) unfolding ssbij_def Tmap_def
-    apply (auto simp: in_context_eqvt supp_inv_bound typ.FFVars_rrenames
-          typ.rrename_comps typ.rrename_comp0s extend_eqvt[symmetric] wf_eqvt Ty_eqvt
-      )
-    done
-  done
-
-lemma fresh: "\<exists>xx. xx \<notin> Tfvars t"
-  by (metis emp_bound equals0D imageI inf.commute inf_absorb2 small_Tfvars small_def small_ssbij subsetI)
-
-lemma swap_idemp[simp]: "id(x := x) = id" by auto
-lemma swap_left: "(id(x := xx, xx := x)) x = xx" by simp
-
-lemma wf_FFVars: "\<turnstile> \<Gamma> ok \<Longrightarrow> a \<in> FFVars_ctxt \<Gamma> \<Longrightarrow> a \<in> dom \<Gamma>"
-  by (induction \<Gamma>) auto
-
-lemma finite_Tfvars: "finite (Tfvars t)"
-using finite_iff_le_card_var small_Tfvars small_def by blast
-
-lemma ls_UNIV_iff_finite: "|A| <o |UNIV::var set| \<longleftrightarrow> finite A"
-using finite_iff_le_card_var by blast
-
-lemma exists_fresh:
-"\<exists> z. z \<notin> set xs \<and> (\<forall>t \<in> set ts. z \<notin> Tfvars t)"
-proof-
-  have 0: "|set xs \<union> \<Union> (Tfvars ` (set ts))| <o |UNIV::var set|" 
-  unfolding ls_UNIV_iff_finite  
-  using finite_Tfvars by blast
-  then obtain x where "x \<notin> set xs \<union> \<Union> (Tfvars ` (set ts))"
-  by (meson exists_fresh) 
-  thus ?thesis by auto
-qed
-
-abbreviation Ii where "Ii \<equiv> \<lambda>(\<Gamma>,S,T). \<Gamma> \<turnstile> S <: T"
-
-lemma rrename_swap_FFvars[simp]: "x \<notin> FFVars_typ T \<Longrightarrow> xx \<notin> FFVars_typ T \<Longrightarrow> 
-  rrename_typ (id(x := xx, xx := x)) T = T"
-apply(rule typ.rrename_cong_ids) by auto
-
-lemma map_context_swap_FFVars[simp]: 
-"\<forall>k\<in>set \<Gamma>. x \<noteq> fst k \<and> x \<notin> FFVars_typ (snd k) \<and> 
-           xx \<noteq> fst k \<and> xx \<notin> FFVars_typ (snd k) \<Longrightarrow> 
-    map_context (id(x := xx, xx := x)) \<Gamma> = \<Gamma>"
-unfolding map_context_def apply(rule map_idI) by auto
-
-lemma G_refresh:
-  "(\<And>t. R t \<Longrightarrow> Ii t) \<Longrightarrow> (\<forall>\<sigma> t. ssbij \<sigma> \<and> R t \<longrightarrow> R (Tmap \<sigma> t)) \<Longrightarrow> small B \<Longrightarrow> G R B t \<Longrightarrow>
-  \<exists>C. small C \<and> C \<inter> Tfvars t = {} \<and> G R C t"
-unfolding G_def Tmap_def apply safe
-  subgoal by (rule exI[of _ "{}"]) auto
-  subgoal by (rule exI[of _ "{}"]) auto
-  subgoal by (rule exI[of _ "{}"]) auto
-  subgoal by (rule exI[of _ "{}"]) fastforce
-  subgoal for \<Gamma> T\<^sub>1 S\<^sub>1 x S\<^sub>2 T\<^sub>2
-  using exists_fresh[of "[x]" "[t]"] apply(elim exE conjE)
-  subgoal for xx apply (rule exI[of _ "{xx}"])
-  apply (intro conjI)
-    subgoal by simp 
-    subgoal by simp 
-    subgoal apply(rule disjI5_5)
-    apply(rule exI[of _ "fst t"])  
-    apply (rule exI[of _ "T\<^sub>1"])
-    apply (rule exI[of _ "S\<^sub>1"])
-    apply (rule exI[of _ "xx"])
-    apply (rule exI[of _ "rrename_typ (id(x:=xx,xx:=x)) S\<^sub>2"])
-    apply (rule exI[of _ "rrename_typ (id(x:=xx,xx:=x)) T\<^sub>2"])
-    apply (cases t) apply simp apply (intro conjI)
-      subgoal apply (subst Forall_rrename[of "id(x:=xx,xx:=x)"]) by auto
-      subgoal apply (subst Forall_rrename[of "id(x:=xx,xx:=x)"]) by auto
-      subgoal for \<Gamma> _ _ apply(erule allE[of _ "id(x:=xx,xx:=x)"])
-      apply(erule allE[of _ "\<Gamma> , x <: T\<^sub>1"])
-      apply(erule allE[of _ S\<^sub>2]) apply(erule allE[of _ T\<^sub>2])
-      subgoal premises P using P(2-)
-      using wf_FFVars[OF wf_context[OF P(1)[OF P(5)]]]
-      wf_context[OF P(1)[OF P(6)]]
-      apply(subgoal_tac "(\<forall>k\<in>set \<Gamma>. x \<noteq> fst k \<and> x \<notin> FFVars_typ (snd k)) \<and> 
-                         x \<notin> FFVars_typ T\<^sub>1")
-      apply(subst (asm) extend_eqvt, simp, simp)
-      subgoal apply (auto simp add: ssbij_def) 
-      by (metis image_eqI map_context_swap_FFVars) 
-      subgoal by (auto simp add: ssbij_def) . . . . . .
-
-(* AtoJ: I also ported the original proof (below), but I think the above 
-one is more maintainable. 
-  using fresh[of t] unfolding G_def Tmap_def apply safe
-  subgoal by (rule exI[of _ "{}"]) auto
-  subgoal by (rule exI[of _ "{}"]) auto
-  subgoal by (rule exI[of _ "{}"]) auto
-  subgoal by (rule exI[of _ "{}"]) fastforce
-  subgoal for xx \<Gamma> T\<^sub>1 S\<^sub>1 x S\<^sub>2 T\<^sub>2
-    apply (rule exI[of _ "{xx}"])
-    apply (rule conjI)
-    subgoal by auto
-    apply(rule conjI, simp) 
-    apply (rule disjI2)+
-    apply (rule exI[of _ "fst t"])
-  apply (rule exI[of _ "T\<^sub>1"])
-    apply (rule exI[of _ "S\<^sub>1"])
-    apply (rule exI[of _ "xx"])
-    apply (rule exI[of _ "rrename_typ (id(x:=xx,xx:=x)) S\<^sub>2"])
-    apply (rule exI[of _ "rrename_typ (id(x:=xx,xx:=x)) T\<^sub>2"])
-    apply (cases t) apply simp
-    apply (intro conjI)
-    subgoal apply (subst Forall_rrename[of "id(x:=xx,xx:=x)"]) by auto
-    subgoal
-      apply (elim conjE)
-        apply (subst Forall_rrename[of "id(x:=xx,xx:=x)"])
-      by auto 
-    subgoal for a b c subgoal premises P
-    using P(2-) apply -
-    apply (rule iffD2[OF arg_cong[of _ _ R]])
-     apply (rule arg_cong[of _ _ "\<lambda>x::\<Gamma>\<^sub>\<tau>. (x, _::type, _::type)"])
-     defer
-     apply (elim allE)
-     apply (erule impE)
-      prefer 2  
-      apply assumption
-     apply (rule conjI)
-      apply (simp add: ssbij_def)
-      apply assumption
-     apply auto[1]
-    apply (subst extend_eqvt)
-      apply (rule bij_swap)
-     apply (rule supp_swap_bound)
-      apply (rule infinite_var)
-    apply (rule arg_cong3[of _ _ _ _ _ _ extend])
-      apply (rule sym)
-      apply (rule context_map_cong_id)
-        apply (rule bij_swap)
-       apply (rule supp_swap_bound)
-       apply (rule infinite_var)
-       apply (erule UnE)
-        apply auto[1]  
-        apply (metis P(1) fst_conv image_eqI wf_ConsE wf_context)
-       apply (drule wf_FFVars[rotated])  
-        apply (meson P(1) wf_context) 
-       apply (metis P(1) fst_conv fun_upd_apply id_apply wf_ConsE wf_context)
-     apply simp
-     apply (smt (verit) P(1) Prelim.bij_swap fst_conv fun_upd_apply 
-       id_apply infinite_var list.discI list.inject subset_eq 
-       supp_swap_bound typ.rrename_cong_ids well_scoped(1) 
-       wf_Ty.cases wf_context) . . . .
-*)
-
-(* The name "PM" of this interpretation stands for "POPLmark" *)
-interpretation PM: Induct1 where dummy = "undefined :: var"
-  and Tmap = Tmap and Tfvars = Tfvars and G = G
-  apply standard
-  using G_mono G_equiv  by auto 
-
-(* AtoJ: Now the proof of this is completely standard, 
-bacause we use the original operator G:  *)
-lemma Ty_PM_I: "Ty \<Gamma> T1 T2 = PM.I (\<Gamma>, T1, T2)"
-unfolding Ty_def PM.I_def lfp_curry3 apply(rule arg_cong2[of _ _ _ _ lfp], simp_all)
-unfolding fun_eq_iff G_def apply clarify
-subgoal for R \<Gamma>\<Gamma> TT1 TT2 apply(rule iffI)
-  subgoal apply(elim disjE exE)
-    \<^cancel>\<open>SA_Top: \<close>
-    subgoal apply(rule exI[of _ "{}"], rule conjI, simp) apply(rule disjI5_1) by auto
-    \<^cancel>\<open>SA_Refl_TVar: \<close>
-    subgoal apply(rule exI[of _ "{}"], rule conjI, simp) apply(rule disjI5_2) by auto
-    \<^cancel>\<open>SA_Trans_TVar: \<close>
-    subgoal apply(rule exI[of _ "{}"], rule conjI, simp) apply(rule disjI5_3) by auto
-    \<^cancel>\<open>SA_Arrow: \<close>
-    subgoal apply(rule exI[of _ "{}"], rule conjI, simp) apply(rule disjI5_4) by auto 
-    \<^cancel>\<open>SA_All: \<close>
-    subgoal for T\<^sub>1 S\<^sub>1 x S\<^sub>2 
-    apply(rule exI[of _ "{x}"], rule conjI, simp) apply(rule disjI5_5) by auto .
-  subgoal apply(elim conjE disjE exE)
-    \<^cancel>\<open>SA_Top: \<close>
-    subgoal apply(rule disjI5_1) by auto
-    \<^cancel>\<open>SA_Refl_TVar: \<close>
-    subgoal apply(rule disjI5_2) by auto
-    \<^cancel>\<open>SA_Trans_TVar: \<close>
-    subgoal apply(rule disjI5_3) by auto
-    \<^cancel>\<open>SA_Arrow: \<close>
-    subgoal apply(rule disjI5_4) by auto 
-    \<^cancel>\<open>SA_All: \<close>
-    subgoal for v \<Gamma> T\<^sub>1 S\<^sub>1 x S\<^sub>2 T\<^sub>2
-    apply(rule disjI5_5) by fastforce . . .
-
-interpretation PM: Induct where dummy = "undefined :: var"
-  and Tmap = Tmap and Tfvars = Tfvars and G = G
-  apply standard subgoal for R B t
-  using G_refresh[of R B t] unfolding Ty_PM_I by auto .
-print_theorems
-
-corollary BE_induct_Ty:
-assumes par: "\<And>p. small (Pfvars p)" 
-and Ty: "\<Gamma> \<turnstile> S <: T" 
-and SA_Top: "\<And>\<Gamma> S p. 
-   \<turnstile> \<Gamma> ok \<Longrightarrow> S closed_in \<Gamma> \<Longrightarrow> 
-   \<phi> p \<Gamma> S Top"
-and SA_Refl_TVar: "\<And>\<Gamma> x p. 
-   \<turnstile> \<Gamma> ok \<Longrightarrow> TyVar x closed_in \<Gamma> \<Longrightarrow> 
-   \<phi> p \<Gamma> (TyVar x) (TyVar x)"
-and SA_Trans_TVar: "\<And>x U \<Gamma> T p. 
-   x <: U \<in> \<Gamma> \<Longrightarrow> \<Gamma> \<turnstile> U <: T \<Longrightarrow> \<forall>p. \<phi> p \<Gamma> U T \<Longrightarrow> 
-   \<phi> p \<Gamma> (TyVar x) T"
-and SA_Arrow: "\<And>\<Gamma> T\<^sub>1 S\<^sub>1 S\<^sub>2 T\<^sub>2 p. 
-   \<Gamma> \<turnstile> T\<^sub>1 <: S\<^sub>1 \<Longrightarrow> \<forall>p. \<phi> p \<Gamma> T\<^sub>1 S\<^sub>1 \<Longrightarrow> \<Gamma> \<turnstile> S\<^sub>2 <: T\<^sub>2 \<Longrightarrow> \<forall>p. \<phi> p \<Gamma> S\<^sub>2 T\<^sub>2 \<Longrightarrow> 
-   \<phi> p \<Gamma> (S\<^sub>1 \<rightarrow> S\<^sub>2) (T\<^sub>1 \<rightarrow> T\<^sub>2)" 
-and SA_All: "\<And>\<Gamma> T\<^sub>1 S\<^sub>1 x S\<^sub>2 T\<^sub>2 p. 
-   x \<notin> Pfvars p \<Longrightarrow> x \<notin> dom \<Gamma> \<Longrightarrow> x \<notin> FFVars_typ S\<^sub>1 \<Longrightarrow> x \<notin> FFVars_typ T\<^sub>1 \<Longrightarrow> 
-   \<Gamma> \<turnstile> T\<^sub>1 <: S\<^sub>1 \<Longrightarrow> \<forall>p. \<phi> p \<Gamma> T\<^sub>1 S\<^sub>1 \<Longrightarrow> \<Gamma> , x <: T\<^sub>1 \<turnstile> S\<^sub>2 <: T\<^sub>2 \<Longrightarrow> 
-   \<forall>p. \<phi> p (\<Gamma> , x <: T\<^sub>1) S\<^sub>2 T\<^sub>2 \<Longrightarrow> 
-   \<phi> p \<Gamma> (\<forall> x <: S\<^sub>1 . S\<^sub>2) (\<forall> x <: T\<^sub>1 . T\<^sub>2)"
-shows "\<phi> p \<Gamma> S T"
-apply(subgoal_tac "case (\<Gamma>, S, T) of (\<Gamma>, S, T) \<Rightarrow> \<phi> p \<Gamma> S T")
-  subgoal by simp
-  subgoal using par Ty
-  apply(elim PM.BE_induct[where R = "\<lambda>p (\<Gamma>, S, T). \<phi> p \<Gamma> S T"])
-    subgoal using Ty_PM_I by simp
-    subgoal for p B t apply(subst (asm) G_def) 
-    unfolding Ty_PM_I[symmetric] apply(elim disjE exE)
-      subgoal using SA_Top by auto
-      subgoal for X using SA_Refl_TVar[of _ X p] by auto
-      subgoal using SA_Trans_TVar by auto
-      subgoal using SA_Arrow by auto
-      subgoal using SA_All by auto . . .
-
 
 (********************* Actual formalization ************************)
 
@@ -601,7 +9,7 @@ ML_file \<open>../../Tools/binder_induction.ML\<close>
 end
 
 (* A bit of customization: *)
-lemma Ty_strong_induct[consumes 1, case_names Bound SA_Top SA_Refl_TVar SA_Trans_TVar SA_Arrow SA_All]:
+lemma ty_strong_induct[consumes 1, case_names Bound SA_Top SA_Refl_TVar SA_Trans_TVar SA_Arrow SA_All]:
   "\<Gamma> \<turnstile> S <: T \<Longrightarrow>
   \<forall>\<rho>. |K \<rho>| <o |UNIV::var set| \<Longrightarrow>
   (\<And>\<Gamma> S \<rho>. \<lbrakk> \<turnstile> \<Gamma> ok ; S closed_in \<Gamma> \<rbrakk> \<Longrightarrow> P \<Gamma> S Top \<rho>) \<Longrightarrow>
@@ -613,31 +21,31 @@ lemma Ty_strong_induct[consumes 1, case_names Bound SA_Top SA_Refl_TVar SA_Trans
       P \<Gamma> (\<forall> x <: S\<^sub>1 . S\<^sub>2) (\<forall> x <: T\<^sub>1 . T\<^sub>2) \<rho>) \<Longrightarrow>
  \<forall>\<rho>. P \<Gamma> S T \<rho>"
 apply safe subgoal for p  
-apply(rule BE_induct_Ty[where \<phi> = "\<lambda> p \<Gamma> S T. P \<Gamma> S T p", of K])
+apply(rule BE_induct_ty[where \<phi> = "\<lambda> p \<Gamma> S T. P \<Gamma> S T p", of K])
 by (auto simp: small_def) .
 
-lemma Ty_refl: "\<lbrakk> \<turnstile> \<Gamma> ok ; T closed_in \<Gamma> \<rbrakk> \<Longrightarrow> \<Gamma> \<turnstile> T <: T"
+lemma ty_refl: "\<lbrakk> \<turnstile> \<Gamma> ok ; T closed_in \<Gamma> \<rbrakk> \<Longrightarrow> \<Gamma> \<turnstile> T <: T"
 proof (binder_induction T arbitrary: \<Gamma> avoiding: "dom \<Gamma>" rule: typ.strong_induct)
   case (TyVar x \<Gamma>)
   then show ?case by blast
 qed (auto simp: Diff_single_insert SA_All wf_Cons)
 
-lemma Ty_permute: "\<lbrakk> \<Gamma> \<turnstile> S <: T ; \<turnstile> \<Delta> ok ; set \<Gamma> = set \<Delta> \<rbrakk> \<Longrightarrow> \<Delta> \<turnstile> S <: T"
-proof (binder_induction \<Gamma> S T arbitrary: \<Delta> avoiding: "dom \<Delta>" rule: Ty_strong_induct)
+lemma ty_permute: "\<lbrakk> \<Gamma> \<turnstile> S <: T ; \<turnstile> \<Delta> ok ; set \<Gamma> = set \<Delta> \<rbrakk> \<Longrightarrow> \<Delta> \<turnstile> S <: T"
+proof (binder_induction \<Gamma> S T arbitrary: \<Delta> avoiding: "dom \<Delta>" rule: ty_strong_induct)
   case (SA_Refl_TVar \<Gamma> x \<Delta>)
   then show ?case by blast
 next
   case (SA_All \<Gamma> T\<^sub>1 S\<^sub>1 x S\<^sub>2 T\<^sub>2 \<Delta>)
   then have "set (\<Gamma>, x <: T\<^sub>1) = set (\<Delta>, x <: T\<^sub>1)" by auto
-  then show ?case by (meson SA_All Ty.SA_All well_scoped(1) wf_Cons)
+  then show ?case by (meson SA_All ty.SA_All well_scoped(1) wf_Cons)
 qed auto
 
 lemma wf_concat: "\<lbrakk> \<turnstile> \<Delta> ok ; \<turnstile> \<Gamma> ok ; \<Gamma> \<bottom> \<Delta> \<rbrakk> \<Longrightarrow> \<turnstile> \<Gamma>,\<Delta> ok"
-proof (induction \<Delta> rule: wf_Ty.induct)
+proof (induction \<Delta> rule: wf_ty.induct)
   case (wf_Cons x \<Delta> T)
   then have 1: "(\<Gamma>, (\<Delta> , x <: T)) = ((\<Gamma>, \<Delta>), x <: T)" by simp
   show ?case unfolding 1
-    apply (rule wf_Ty.wf_Cons)
+    apply (rule wf_ty.wf_Cons)
     using wf_Cons by auto
 qed auto
 
@@ -648,30 +56,30 @@ lemma wf_concat_disjoint: "\<turnstile> \<Gamma>, \<Delta> ok \<Longrightarrow> 
 proof (induction \<Delta>)
   case (Cons a \<Delta>)
   then show ?case
-    by (smt (verit, del_insts) Un_iff append_Cons disjoint_iff fst_conv image_iff inf.idem insertE list.inject list.simps(15) set_append set_empty2 wf_Ty.cases)
+    by (smt (verit, del_insts) Un_iff append_Cons disjoint_iff fst_conv image_iff inf.idem insertE list.inject list.simps(15) set_append set_empty2 wf_ty.cases)
 qed simp
 
 lemma wf_insert: "\<lbrakk> \<turnstile> \<Gamma>,\<Delta> ok ; x \<notin> dom \<Gamma> ; x \<notin> dom \<Delta> ; T closed_in \<Gamma> \<rbrakk> \<Longrightarrow> \<turnstile> \<Gamma>,x<:T,\<Delta> ok"
   by (induction \<Delta>) auto
 
-lemma Ty_weakening: "\<lbrakk> \<Gamma> \<turnstile> S <: T ; \<turnstile> \<Gamma>,\<Delta> ok \<rbrakk> \<Longrightarrow> \<Gamma>,\<Delta> \<turnstile> S <: T"
-proof (binder_induction \<Gamma> S T avoiding: "dom \<Delta>" rule: Ty_strong_induct)
+lemma ty_weakening: "\<lbrakk> \<Gamma> \<turnstile> S <: T ; \<turnstile> \<Gamma>,\<Delta> ok \<rbrakk> \<Longrightarrow> \<Gamma>,\<Delta> \<turnstile> S <: T"
+proof (binder_induction \<Gamma> S T avoiding: "dom \<Delta>" rule: ty_strong_induct)
   case (SA_Top \<Gamma> S)
-  then show ?case using Ty.SA_Top weaken_closed wf_concat_disjoint by presburger
+  then show ?case using ty.SA_Top weaken_closed wf_concat_disjoint by presburger
 next
   case (SA_Refl_TVar \<Gamma> x)
-  then show ?case using Ty.SA_Refl_TVar weaken_closed wf_concat_disjoint by presburger
+  then show ?case using ty.SA_Refl_TVar weaken_closed wf_concat_disjoint by presburger
 next
   case (SA_All \<Gamma> T\<^sub>1 S\<^sub>1 x S\<^sub>2 T\<^sub>2)
   have 1: "\<turnstile> \<Gamma>, x <: T\<^sub>1, \<Delta> ok"
     by (meson wf_insert SA_All.hyps(1,2,5) SA_All.prems well_scoped(1)) 
   have 2: "\<turnstile> \<Gamma> , \<Delta> , x <: T\<^sub>1 ok"
     by (smt (verit, del_insts) SA_All(1,6,7,9) UnE fst_conv image_iff set_append well_scoped(1) wf_Cons wf_ConsE wf_context)
-  show ?case using Ty_permute[OF _ 2] 1 SA_All by auto
+  show ?case using ty_permute[OF _ 2] 1 SA_All by auto
 qed auto
 
-corollary Ty_weakening_extend: "\<lbrakk> \<Gamma> \<turnstile> S <: T ; X \<notin> dom \<Gamma> ; Q closed_in \<Gamma> \<rbrakk> \<Longrightarrow> \<Gamma>,X<:Q \<turnstile> S <: T"
-  using Ty_weakening[of _ _ _ "[(X, Q)]"] by (metis append_Cons append_Nil wf_Cons wf_context)
+corollary ty_weakening_extend: "\<lbrakk> \<Gamma> \<turnstile> S <: T ; X \<notin> dom \<Gamma> ; Q closed_in \<Gamma> \<rbrakk> \<Longrightarrow> \<Gamma>,X<:Q \<turnstile> S <: T"
+  using ty_weakening[of _ _ _ "[(X, Q)]"] by (metis append_Cons append_Nil wf_Cons wf_context)
 
 lemma wf_concatD: "\<turnstile> \<Gamma>, \<Delta> ok \<Longrightarrow> \<turnstile> \<Gamma> ok"
   by (induction \<Delta>) auto
@@ -689,7 +97,7 @@ proof (induction \<Delta>)
   then have "\<turnstile> \<Gamma>, X <: R, \<Delta> ok" by auto
   obtain b c where 2: "a = (b, c)" by fastforce
   then have 1: "\<And>R. \<Gamma> , X <: R, (a # \<Delta>) = (b, c) # (\<Gamma> , X <: R, \<Delta>)" by simp
-  have "b \<notin> POPLmark_1A.dom (\<Gamma> , X <: R, \<Delta>)" using Cons(2)[unfolded 1] by auto
+  have "b \<notin> dom (\<Gamma> , X <: R, \<Delta>)" using Cons(2)[unfolded 1] by auto
   then show ?case unfolding 1 using Cons 2 by auto
 qed auto
 
@@ -700,7 +108,7 @@ lemma SA_AllE1[consumes 2, case_names SA_Trans_TVar SA_All]:
     and Top: "\<And>\<Gamma>. \<lbrakk> \<turnstile> \<Gamma> ok ; \<forall>X<:S\<^sub>1. S\<^sub>2 closed_in \<Gamma> \<rbrakk> \<Longrightarrow> R \<Gamma> (\<forall>X<:S\<^sub>1. S\<^sub>2) Top"
     and Forall: "\<And>\<Gamma> T\<^sub>1 T\<^sub>2. \<lbrakk> \<Gamma> \<turnstile> T\<^sub>1 <: S\<^sub>1 ; \<Gamma>, X<:T\<^sub>1 \<turnstile> S\<^sub>2 <: T\<^sub>2 \<rbrakk> \<Longrightarrow> R \<Gamma> (\<forall>X<:S\<^sub>1. S\<^sub>2) (\<forall>X<:T\<^sub>1 . T\<^sub>2)"
   shows "R \<Gamma> (\<forall>X<:S\<^sub>1. S\<^sub>2) T"
-using assms(1,2) proof (binder_induction \<Gamma> "\<forall>X<:S\<^sub>1. S\<^sub>2" T rule: Ty_strong_induct)
+using assms(1,2) proof (binder_induction \<Gamma> "\<forall>X<:S\<^sub>1. S\<^sub>2" T rule: ty_strong_induct)
   case (SA_All \<Gamma> T\<^sub>1 R\<^sub>1 Y R\<^sub>2 T\<^sub>2)
   have 1: "\<forall>Y<:T\<^sub>1 . T\<^sub>2 = \<forall>X<:T\<^sub>1. rrename_typ (id(Y:=X,X:=Y)) T\<^sub>2"
     apply (rule Forall_swap)
@@ -717,8 +125,8 @@ using assms(1,2) proof (binder_induction \<Gamma> "\<forall>X<:S\<^sub>1. S\<^su
   show ?case unfolding 1
     apply (rule Forall)
     using same SA_All(5) apply simp
-    apply (rule iffD2[OF arg_cong3[OF _ _ refl, of _ _ _ _ Ty], rotated -1])
-      apply (rule Ty_eqvt)
+    apply (rule iffD2[OF arg_cong3[OF _ _ refl, of _ _ _ _ ty], rotated -1])
+      apply (rule ty_eqvt)
         apply (rule SA_All(7))
        apply (rule bij_swap supp_swap_bound infinite_var)+
      apply (subst extend_eqvt)
@@ -736,7 +144,7 @@ lemma SA_AllE2[consumes 2, case_names SA_Trans_TVar SA_All]:
     and TyVar: "\<And>\<Gamma> x U. \<lbrakk> x<:U \<in> \<Gamma> ; \<Gamma> \<turnstile> U <: \<forall> X <: T\<^sub>1 . T\<^sub>2 ; R \<Gamma> U (\<forall>X<:T\<^sub>1. T\<^sub>2) \<rbrakk> \<Longrightarrow> R \<Gamma> (TyVar x) (\<forall> X <: T\<^sub>1 . T\<^sub>2)"
     and Forall: "\<And>\<Gamma> S\<^sub>1 S\<^sub>2. \<lbrakk> \<Gamma> \<turnstile> T\<^sub>1 <: S\<^sub>1 ; \<Gamma>, X<:T\<^sub>1 \<turnstile> S\<^sub>2 <: T\<^sub>2 \<rbrakk> \<Longrightarrow> R \<Gamma> (\<forall>X<:S\<^sub>1. S\<^sub>2) (\<forall> X <: T\<^sub>1 . T\<^sub>2)"
   shows "R \<Gamma> S (\<forall>X<:T\<^sub>1. T\<^sub>2)"
-using assms(1,2) proof (binder_induction \<Gamma> S "\<forall>X<:T\<^sub>1. T\<^sub>2" rule: Ty_strong_induct)
+using assms(1,2) proof (binder_induction \<Gamma> S "\<forall>X<:T\<^sub>1. T\<^sub>2" rule: ty_strong_induct)
   case (SA_All \<Gamma> R\<^sub>1 S\<^sub>1 Y S\<^sub>2 R\<^sub>2)
   have 1: "\<forall>Y<:S\<^sub>1. S\<^sub>2 = \<forall>X<:S\<^sub>1. rrename_typ (id(Y:=X,X:=Y)) S\<^sub>2"
     apply (rule Forall_swap)
@@ -754,8 +162,8 @@ using assms(1,2) proof (binder_induction \<Gamma> S "\<forall>X<:T\<^sub>1. T\<^
   show ?case unfolding 1
     apply (rule Forall)
      apply (metis SA_All(5,9) typ_inject(3))
-    apply (rule iffD2[OF arg_cong3[OF _ refl, of _ _ _ _ Ty], rotated -1])
-      apply (rule Ty_eqvt)
+    apply (rule iffD2[OF arg_cong3[OF _ refl, of _ _ _ _ ty], rotated -1])
+      apply (rule ty_eqvt)
         apply (rule SA_All(7))
        apply (rule bij_swap supp_swap_bound infinite_var)+
      apply (subst extend_eqvt)
@@ -767,23 +175,23 @@ using assms(1,2) proof (binder_induction \<Gamma> S "\<forall>X<:T\<^sub>1. T\<^
     using SA_All(9) x Forall_inject_same unfolding same by simp
 qed (auto simp: TyVar)
 
-lemma Ty_transitivity : "\<lbrakk> \<Gamma> \<turnstile> S <: Q ; \<Gamma> \<turnstile> Q <: T \<rbrakk> \<Longrightarrow> \<Gamma> \<turnstile> S <: T"
-  and Ty_narrowing : "\<lbrakk> (\<Gamma> , X <: Q), \<Delta> \<turnstile> M <: N ; \<Gamma> \<turnstile> R <: Q \<rbrakk> \<Longrightarrow> (\<Gamma>, X <: R), \<Delta> \<turnstile> M <: N"
+lemma ty_transitivity : "\<lbrakk> \<Gamma> \<turnstile> S <: Q ; \<Gamma> \<turnstile> Q <: T \<rbrakk> \<Longrightarrow> \<Gamma> \<turnstile> S <: T"
+  and ty_narrowing : "\<lbrakk> (\<Gamma> , X <: Q), \<Delta> \<turnstile> M <: N ; \<Gamma> \<turnstile> R <: Q \<rbrakk> \<Longrightarrow> (\<Gamma>, X <: R), \<Delta> \<turnstile> M <: N"
 proof -
   have
-    Ty_trans: "\<lbrakk> \<Gamma> \<turnstile> S <: Q ; \<Gamma> \<turnstile> Q <: T \<rbrakk> \<Longrightarrow> \<Gamma> \<turnstile> S <: T"
-  and Ty_narrow: "\<lbrakk> (\<Gamma> , X <: Q), \<Delta> \<turnstile> M <: N ; \<Gamma> \<turnstile> R <: Q ; \<turnstile> \<Gamma> , X <: R, \<Delta> ok ; M closed_in \<Gamma> , X <: R, \<Delta> ; N closed_in \<Gamma> , X <: R, \<Delta> \<rbrakk> \<Longrightarrow> (\<Gamma>, X <: R), \<Delta> \<turnstile> M <: N"
+    ty_trans: "\<lbrakk> \<Gamma> \<turnstile> S <: Q ; \<Gamma> \<turnstile> Q <: T \<rbrakk> \<Longrightarrow> \<Gamma> \<turnstile> S <: T"
+  and ty_narrow: "\<lbrakk> (\<Gamma> , X <: Q), \<Delta> \<turnstile> M <: N ; \<Gamma> \<turnstile> R <: Q ; \<turnstile> \<Gamma> , X <: R, \<Delta> ok ; M closed_in \<Gamma> , X <: R, \<Delta> ; N closed_in \<Gamma> , X <: R, \<Delta> \<rbrakk> \<Longrightarrow> (\<Gamma>, X <: R), \<Delta> \<turnstile> M <: N"
   proof (binder_induction Q arbitrary: \<Gamma> \<Delta> S T M N X R avoiding: X "dom \<Gamma>" "dom \<Delta>" rule: typ.strong_induct)
     case (TyVar Y \<Gamma> \<Delta> S T M N X R)
     {
       fix \<Gamma> S T
-      show Ty_trans: "\<Gamma> \<turnstile> S <: TyVar Y \<Longrightarrow> \<Gamma> \<turnstile> TyVar Y <: T \<Longrightarrow> \<Gamma> \<turnstile> S <: T"
-        by (induction \<Gamma> S "TyVar Y" rule: Ty.induct) auto
-    } note Ty_trans = this
+      show ty_trans: "\<Gamma> \<turnstile> S <: TyVar Y \<Longrightarrow> \<Gamma> \<turnstile> TyVar Y <: T \<Longrightarrow> \<Gamma> \<turnstile> S <: T"
+        by (induction \<Gamma> S "TyVar Y" rule: ty.induct) auto
+    } note ty_trans = this
     {
       case 2
       then show ?case
-      proof (binder_induction "\<Gamma>, X <: TyVar Y, \<Delta>" M N arbitrary: \<Delta> avoiding: X "dom \<Gamma>" "dom \<Delta>" rule: Ty_strong_induct)
+      proof (binder_induction "\<Gamma>, X <: TyVar Y, \<Delta>" M N arbitrary: \<Delta> avoiding: X "dom \<Gamma>" "dom \<Delta>" rule: ty_strong_induct)
         case (SA_Trans_TVar Z U T \<Delta>')
         show ?case
         proof (cases "X = Z")
@@ -791,15 +199,15 @@ proof -
           then have u: "U = TyVar Y" using SA_Trans_TVar(1,2) context_determ wf_context by blast
           have "TyVar Y closed_in \<Gamma>, Z <: R, \<Delta>'" using SA_Trans_TVar(2) True u well_scoped(1) by fastforce
           then have "\<Gamma> , Z <: R , \<Delta>' \<turnstile> TyVar Y <: T" using SA_Trans_TVar True u by auto
-          moreover have "\<Gamma>, Z <: R, \<Delta>' \<turnstile> R <: TyVar Y" using Ty_weakening[OF Ty_weakening_extend[OF SA_Trans_TVar(4)]]
+          moreover have "\<Gamma>, Z <: R, \<Delta>' \<turnstile> R <: TyVar Y" using ty_weakening[OF ty_weakening_extend[OF SA_Trans_TVar(4)]]
             by (metis SA_Trans_TVar.prems(2) True wf_ConsE wf_concatD)
-          ultimately have "\<Gamma> , Z <: R , \<Delta>' \<turnstile> R <: T" using Ty_trans by blast
-          then show ?thesis unfolding True u using Ty.SA_Trans_TVar by auto
+          ultimately have "\<Gamma> , Z <: R , \<Delta>' \<turnstile> R <: T" using ty_trans by blast
+          then show ?thesis unfolding True u using ty.SA_Trans_TVar by auto
         next
           case False
           have x: "U closed_in \<Gamma> , X <: R , \<Delta>'" using SA_Trans_TVar(2) well_scoped(1) by fastforce
           show ?thesis
-            apply (rule Ty.SA_Trans_TVar)
+            apply (rule ty.SA_Trans_TVar)
             using SA_Trans_TVar False x by auto
         qed
       next
@@ -818,11 +226,11 @@ proof -
     }
   next
     case (Top \<Gamma> \<Delta> S T M N X R)
-    show Ty_trans: "\<Gamma> \<turnstile> S <: Top \<Longrightarrow> \<Gamma> \<turnstile> Top <: T \<Longrightarrow> \<Gamma> \<turnstile> S <: T" by auto
+    show ty_trans: "\<Gamma> \<turnstile> S <: Top \<Longrightarrow> \<Gamma> \<turnstile> Top <: T \<Longrightarrow> \<Gamma> \<turnstile> S <: T" by auto
     {
       case 2
       then show ?case
-      proof (binder_induction "\<Gamma>, X <: Top, \<Delta>" M N arbitrary: \<Delta> avoiding: X "dom \<Gamma>" "dom \<Delta>" rule: Ty_strong_induct)
+      proof (binder_induction "\<Gamma>, X <: Top, \<Delta>" M N arbitrary: \<Delta> avoiding: X "dom \<Gamma>" "dom \<Delta>" rule: ty_strong_induct)
         case (SA_Trans_TVar Z U T \<Delta>')
         then show ?case
         proof (cases "X = Z")
@@ -830,13 +238,13 @@ proof -
           then have u: "U = Top" using SA_Trans_TVar(1,2) context_determ wf_context by blast
           have "\<Gamma> , Z <: R , \<Delta>' \<turnstile> Top <: T" using SA_Trans_TVar True u by auto
           then have "\<Gamma> , Z <: R , \<Delta>' \<turnstile> R <: T"
-            by (metis SA_TopE SA_Trans_TVar.prems(1) Ty_weakening Ty_weakening_extend wf_ConsE wf_concatD)
-          then show ?thesis unfolding True u using Ty.SA_Trans_TVar by auto
+            by (metis SA_TopE SA_Trans_TVar.prems(1) ty_weakening ty_weakening_extend wf_ConsE wf_concatD)
+          then show ?thesis unfolding True u using ty.SA_Trans_TVar by auto
         next
           case False
           have x: "U closed_in \<Gamma> , X <: R , \<Delta>'" using SA_Trans_TVar(2) well_scoped(1) by fastforce
           show ?thesis
-            apply (rule Ty.SA_Trans_TVar)
+            apply (rule ty.SA_Trans_TVar)
             using SA_Trans_TVar False x by auto
         qed
       next
@@ -859,22 +267,22 @@ proof -
       fix \<Gamma> S T
       assume "\<Gamma> \<turnstile> S <: Q\<^sub>1 \<rightarrow> Q\<^sub>2" "\<Gamma> \<turnstile> Q\<^sub>1 \<rightarrow> Q\<^sub>2 <: T"
       then show "\<Gamma> \<turnstile> S <: T"
-      proof (induction \<Gamma> S "Q\<^sub>1 \<rightarrow> Q\<^sub>2" rule: Ty.induct)
+      proof (induction \<Gamma> S "Q\<^sub>1 \<rightarrow> Q\<^sub>2" rule: ty.induct)
         case left: (SA_Arrow \<Gamma> T\<^sub>1 S\<^sub>1 S\<^sub>2 T\<^sub>2)
         from left(6,1-5) show ?case
         proof cases
           case SA_Top
-          then show ?thesis by (meson left(1,3) Ty.SA_Arrow Ty.SA_Top well_scoped(1))
+          then show ?thesis by (meson left(1,3) ty.SA_Arrow ty.SA_Top well_scoped(1))
         next
           case right: (SA_Arrow U\<^sub>1 R\<^sub>1 R\<^sub>2 U\<^sub>2)
           then show ?thesis using left by (metis Fun(1,3) SA_Arrow typ_inject(2))
         qed auto
       qed auto
-    } note Ty_trans = this
+    } note ty_trans = this
     {
       case 2
       then show ?case
-      proof (binder_induction "\<Gamma>, X <: (Q\<^sub>1 \<rightarrow> Q\<^sub>2), \<Delta>" M N arbitrary: \<Delta> avoiding: X "dom \<Gamma>" "dom \<Delta>" rule: Ty_strong_induct)
+      proof (binder_induction "\<Gamma>, X <: (Q\<^sub>1 \<rightarrow> Q\<^sub>2), \<Delta>" M N arbitrary: \<Delta> avoiding: X "dom \<Gamma>" "dom \<Delta>" rule: ty_strong_induct)
         case (SA_Trans_TVar Z U T \<Delta>')
         then show ?case
         proof (cases "X = Z")
@@ -882,15 +290,15 @@ proof -
           then have u: "U = (Q\<^sub>1 \<rightarrow> Q\<^sub>2)" using SA_Trans_TVar(1,2) context_determ wf_context by blast
           have "(Q\<^sub>1 \<rightarrow> Q\<^sub>2) closed_in \<Gamma>, Z <: R, \<Delta>'" using SA_Trans_TVar(2) True u well_scoped(1) by fastforce
           then have "\<Gamma> , Z <: R , \<Delta>' \<turnstile> (Q\<^sub>1 \<rightarrow> Q\<^sub>2) <: T" using SA_Trans_TVar True u by auto
-          moreover have "\<Gamma>, Z <: R, \<Delta>' \<turnstile> R <: (Q\<^sub>1 \<rightarrow> Q\<^sub>2)" using Ty_weakening[OF Ty_weakening_extend[OF SA_Trans_TVar(4)]]
+          moreover have "\<Gamma>, Z <: R, \<Delta>' \<turnstile> R <: (Q\<^sub>1 \<rightarrow> Q\<^sub>2)" using ty_weakening[OF ty_weakening_extend[OF SA_Trans_TVar(4)]]
             by (metis SA_Trans_TVar.prems(2) True wf_ConsE wf_concatD)
-          ultimately have "\<Gamma> , Z <: R , \<Delta>' \<turnstile> R <: T" using Ty_trans by blast
-          then show ?thesis unfolding True u using Ty.SA_Trans_TVar by auto
+          ultimately have "\<Gamma> , Z <: R , \<Delta>' \<turnstile> R <: T" using ty_trans by blast
+          then show ?thesis unfolding True u using ty.SA_Trans_TVar by auto
         next
           case False
           have x: "U closed_in \<Gamma> , X <: R , \<Delta>'" using SA_Trans_TVar(2) well_scoped(1) by fastforce
           show ?thesis
-            apply (rule Ty.SA_Trans_TVar)
+            apply (rule ty.SA_Trans_TVar)
             using SA_Trans_TVar False x by auto
         qed
       next
@@ -909,7 +317,7 @@ proof -
     }
   next
     case (Forall X Q\<^sub>1 Q\<^sub>2 \<Gamma> \<Delta> S T M N Y R)
-    have Ty_trans: "\<And>\<Gamma> S T. X \<notin> dom \<Gamma> \<Longrightarrow> \<Gamma> \<turnstile> S <: \<forall>X<:Q\<^sub>1. Q\<^sub>2 \<Longrightarrow> \<Gamma> \<turnstile> \<forall>X<:Q\<^sub>1. Q\<^sub>2 <: T \<Longrightarrow> \<Gamma> \<turnstile> S <: T"
+    have ty_trans: "\<And>\<Gamma> S T. X \<notin> dom \<Gamma> \<Longrightarrow> \<Gamma> \<turnstile> S <: \<forall>X<:Q\<^sub>1. Q\<^sub>2 \<Longrightarrow> \<Gamma> \<turnstile> \<forall>X<:Q\<^sub>1. Q\<^sub>2 <: T \<Longrightarrow> \<Gamma> \<turnstile> S <: T"
     proof -
       fix \<Gamma> S T
       assume a: "X \<notin> dom \<Gamma>" "\<Gamma> \<turnstile> S <: \<forall>X<:Q\<^sub>1. Q\<^sub>2" "\<Gamma> \<turnstile> \<forall>X<:Q\<^sub>1. Q\<^sub>2 <: T"
@@ -919,7 +327,7 @@ proof -
         from SA_All(3,4,1,2) show ?case
         proof (induction rule: SA_AllE1)
           case (SA_Trans_TVar \<Gamma>)
-          then show ?case by (meson SA_Top Ty.SA_All well_scoped(1))
+          then show ?case by (meson SA_Top ty.SA_All well_scoped(1))
         next
           case (SA_All \<Gamma> T\<^sub>1 T\<^sub>2)
           have 1: "\<Gamma> \<turnstile> T\<^sub>1 <: S\<^sub>1" by (rule Forall(2)[OF SA_All(1,3)])
@@ -932,11 +340,11 @@ proof -
     qed
     {
       case 1
-      then show ?case using Ty_trans Forall(1) by blast
+      then show ?case using ty_trans Forall(1) by blast
     next
       case 2
       then show ?case using Forall(1)
-      proof (binder_induction "\<Gamma>, Y <: (\<forall>X<:Q\<^sub>1. Q\<^sub>2), \<Delta>" M N arbitrary: \<Delta> avoiding: X Y "dom \<Gamma>" "dom \<Delta>" rule: Ty_strong_induct)
+      proof (binder_induction "\<Gamma>, Y <: (\<forall>X<:Q\<^sub>1. Q\<^sub>2), \<Delta>" M N arbitrary: \<Delta> avoiding: X Y "dom \<Gamma>" "dom \<Delta>" rule: ty_strong_induct)
         case (SA_Trans_TVar Z U T \<Delta>')
         then show ?case
         proof (cases "Y = Z")
@@ -944,16 +352,16 @@ proof -
           then have u: "U = \<forall> X <: Q\<^sub>1 . Q\<^sub>2" using SA_Trans_TVar(1,2) context_determ wf_context by blast
           have "\<forall> X <: Q\<^sub>1 . Q\<^sub>2 closed_in \<Gamma>, Z <: R, \<Delta>'" using SA_Trans_TVar(2) True u well_scoped(1) by fastforce
           then have "\<Gamma> , Z <: R , \<Delta>' \<turnstile> \<forall> X <: Q\<^sub>1 . Q\<^sub>2 <: T" using SA_Trans_TVar True u by auto
-          moreover have "\<Gamma>, Z <: R, \<Delta>' \<turnstile> R <: \<forall> X <: Q\<^sub>1 . Q\<^sub>2" using Ty_weakening[OF Ty_weakening_extend[OF SA_Trans_TVar(4)]]
+          moreover have "\<Gamma>, Z <: R, \<Delta>' \<turnstile> R <: \<forall> X <: Q\<^sub>1 . Q\<^sub>2" using ty_weakening[OF ty_weakening_extend[OF SA_Trans_TVar(4)]]
             by (metis SA_Trans_TVar.prems(2) True wf_ConsE wf_concatD)
           moreover have "X \<notin> dom (\<Gamma> , Z <: R , \<Delta>')" using SA_Trans_TVar(8) True by auto
-          ultimately have "\<Gamma>, Z <: R, \<Delta>' \<turnstile> R <: T" using Ty_trans by blast
-          then show ?thesis unfolding True u using Ty.SA_Trans_TVar by auto
+          ultimately have "\<Gamma>, Z <: R, \<Delta>' \<turnstile> R <: T" using ty_trans by blast
+          then show ?thesis unfolding True u using ty.SA_Trans_TVar by auto
         next
           case False
           have x: "U closed_in \<Gamma> , Y <: R , \<Delta>'" using SA_Trans_TVar(2) well_scoped(1) by fastforce
           show ?thesis
-            apply (rule Ty.SA_Trans_TVar)
+            apply (rule ty.SA_Trans_TVar)
             using SA_Trans_TVar False x by auto
         qed
       next
@@ -971,14 +379,12 @@ proof -
     }
   qed simp_all
 
-  show "\<lbrakk> \<Gamma> \<turnstile> S <: Q ; \<Gamma> \<turnstile> Q <: T \<rbrakk> \<Longrightarrow> \<Gamma> \<turnstile> S <: T" using Ty_trans by blast
+  show "\<lbrakk> \<Gamma> \<turnstile> S <: Q ; \<Gamma> \<turnstile> Q <: T \<rbrakk> \<Longrightarrow> \<Gamma> \<turnstile> S <: T" using ty_trans by blast
   show "\<lbrakk> (\<Gamma> , X <: Q), \<Delta> \<turnstile> M <: N ; \<Gamma> \<turnstile> R <: Q \<rbrakk> \<Longrightarrow> (\<Gamma>, X <: R), \<Delta> \<turnstile> M <: N"
-    apply (rule Ty_narrow)
+    apply (rule ty_narrow)
         apply assumption+
     using narrow_wf well_scoped wf_context apply metis
     using well_scoped by fastforce+
 qed
 
-(**)
-
-end
+end 
